Change hashmaps to work with tagged blocks via opaque encoding function.

src/PermAsyncDisk.v
@@ -103,11 +103,22 @@ Definition rawdisk := @mem addr addr_eq_dec valuset.
 Definition vsmerge (vs : valuset) : list tagged_block := fst vs :: snd vs.
 
 
+
+(* Encoding of tagged blocks for hashing purposes *)
+Parameter encoding_length: nat.
+Parameter encode: tagged_block -> word encoding_length.
+Parameter decode: word encoding_length -> tagged_block.
+Axiom encode_inj: forall b1 b2, encode b1 = encode b2 <-> b1 = b2.
+Axiom decode_inj: forall w1 w2, decode w1 = decode w2 <-> w1 = w2.
+Axiom encode_decode: forall b, decode (encode b) = b.
+Axiom decode_encode: forall w, encode (decode w) = w.
+
 (* Hashing *)
 Definition hashlen := 32.
 Parameter hash_fwd : forall sz, word sz -> word hashlen.
-Definition default_valu : valu := $0.
-Definition default_hash := hash_fwd default_valu.
+(* Definition default_valu : valu := $0. *)
+Definition default_encoding := encode tagged_block0.
+Definition default_hash := hash_fwd (encode tagged_block0).
 
 (* A hashmap holds all keys that Hash has been called on, maps hash values to keys. *)
 Inductive hashmap : Type :=
@@ -119,7 +130,7 @@ Definition upd_hashmap' hm h sz k : hashmap :=
 
 Fixpoint hashmap_get hm h : option {sz : nat & word sz} :=
   if (weq h default_hash)
-    then Some (existT _ _ default_valu) else
+    then Some (existT _ _ default_encoding) else
     (match hm with
     | empty_hashmap => None
     | upd_hashmap hm' h' k' =>  if (weq h' h)
